program_logic/sts.v
@@ -3,12 +3,12 @@ From program_logic Require Export invariants global_functor.
 Import uPred.
 
 Class stsG Λ Σ (sts : stsT) := StsG {
-  sts_inG :> inG Λ Σ (stsRA sts);
+  sts_inG :> inG Λ Σ (stsR sts);
   sts_inhabited :> Inhabited (sts.state sts);
 }.
 Coercion sts_inG : stsG >-> inG.
 
-Definition stsGF (sts : stsT) : iFunctor := constF (stsRA sts).
+Definition stsGF (sts : stsT) : iFunctor := constF (stsR sts).
 Instance inGF_stsG sts `{inGF Λ Σ (stsGF sts)}
   `{Inhabited (sts.state sts)} : stsG Λ Σ sts.
 Proof. split; try apply _. apply: inGF_inG. Qed.
